maker.sh
@@ -4,4 +4,5 @@ coqc CrushEquality.v &&
 coqc MyShortHand.v &&
 coqc ProtoSynthDataTypes.v &&
 coqc ProtoSynthProtocolDataTypes.v &&
-coqc TrueProtoSynth.v
+coqc TrueProtoSynth.v &&
+coqc TrueProtoSynth2.v
